open import Data.String as String using (String; fromList)
open import Data.Nat              using (ℕ; zero; suc; _+_; _*_;  _<′_; _≤′_)
open import Data.Nat.Properties  
open import Data.Bool             using (Bool; true; false; if_then_else_)
open import Data.List   hiding (merge; partition)
open import Data.List.Properties  using (map-id; map-compose)
open import Data.Product          using (Σ; Σ-syntax; _,_; proj₁; proj₂; _×_; map)
open import Data.Sum   as Sum     using (_⊎_; inj₁; inj₂; map)
open import Data.Unit             using (⊤; tt)
open import Data.Empty            using (⊥; ⊥-elim)
open import Relation.Binary.PropositionalEquality
  using (_≡_; refl; cong; cong₂; cong-app; sym; trans; subst; module ≡-Reasoning)
open ≡-Reasoning
open import Relation.Nullary      using (¬_; Dec; yes; no)
open import Induction.WellFounded
open import Relation.Binary
open import Data.Nat.Induction

data _≤_ : ℕ  -> ℕ -> Set where
  ≤-reflex : {n : ℕ } -> n ≤ n
  s≤s : {n m : ℕ } -> ( n ≤ m ) -> (  n  ≤  suc m )

zero≤n : ( n : ℕ )  -> zero ≤ n
zero≤n zero = ≤-reflex
zero≤n (suc n) = s≤s (zero≤n n)

transitive : { n m o : ℕ } -> n ≤ m -> m ≤ o -> n ≤ o
transitive {n} {.n} {o} ≤-reflex x₁ = x₁
transitive {n} {.(suc _)} {.(suc _)} (s≤s x) ≤-reflex = s≤s x
transitive {n} {.(suc _)} {.(suc _)} (s≤s x) (s≤s x₁) = s≤s (transitive x (transitive (s≤s ≤-reflex) x₁))

sucsuc : (n m : ℕ ) -> n ≤ m -> (suc n ) ≤ (suc m )
sucsuc n .n ≤-reflex = ≤-reflex
sucsuc n .(suc m) (s≤s {m = m} x) = transitive (sucsuc _ _ x) (s≤s ≤-reflex)

em : ( m n : ℕ ) -> ( m ≤ n ) ⊎ ( n ≤ m )
em zero n = inj₁ (zero≤n n)
em (suc m) zero = inj₂ (zero≤n (suc m))
em (suc m) (suc n) with em m n
em (suc m) (suc n) | inj₁ x = inj₁ (sucsuc _ _ x)
em (suc m) (suc n) | inj₂ y = inj₂ (sucsuc _ _ y)

≤reflrefl : {m n : ℕ} -> m ≤ n -> n ≤ m -> m ≡ n
≤reflrefl {m} {.m} ≤-reflex x₁ = refl
≤reflrefl {.(suc _)} {.(suc _)} (s≤s x) ≤-reflex = refl
≤reflrefl {.(suc m)} {.(suc _)} (s≤s x) (s≤s {m = m} x₁) with transitive (s≤s ≤-reflex) x₁ |  transitive (s≤s ≤-reflex) x
≤reflrefl {.(suc m)} {.(suc _)} (s≤s x) (s≤s {m = m} x₁) | a | b = cong suc (≤reflrefl b a)
  
data sorted : List ℕ -> Set where
  nil : sorted []
  one : {x : ℕ } -> sorted ( x ∷ [] )
  two : (x y : ℕ ) -> (L : List ℕ ) -> x ≤ y -> sorted ( y ∷ L ) -> sorted ( x ∷ y ∷ L )

{-
{- https://stackoverflow.com/questions/17910737/termination-check-on-list-merge/17912550#17912550 -}
merge : List ℕ -> List ℕ -> List ℕ
merge [] x₁ = x₁
merge (x ∷ x₂) [] = x ∷ x₂ 
merge (x ∷ xs) (y ∷ ys) with em x y | merge xs (y ∷ ys ) | merge  (x ∷ xs )  ys
merge (x ∷ xs) (y ∷ ys) | inj₁ x₁ | b | c = x ∷ b
merge (x ∷ xs) (y ∷ ys) | inj₂ y₁ | b | c = y ∷ c 
-}

{-
{- the third way to define merge -}
merge-aux : {x y : ℕ} ->  ( x ≤ y ) ⊎ (y ≤ x )  -> List ℕ -> List ℕ -> List ℕ
merge-aux (inj₁ x) x₁ x₂ = x₁
merge-aux (inj₂ y) x₁ x₂ = x₂

merge : List ℕ -> List ℕ -> List ℕ
merge [] x₁ = x₁
merge (x ∷ x₂) [] = x ∷ x₂
merge (x ∷ x₂) (x₁ ∷ x₃) = merge-aux (em x x₁) (x ∷ merge x₂ (x₁ ∷ x₃)) (x₁ ∷ merge (x ∷ x₂)  x₃)
-}

{- the fourth way to define merge -}
merge : List ℕ -> List ℕ -> List ℕ
merge [] x₁ = x₁
merge (x ∷ x₂) [] = x ∷ x₂ 
merge (x ∷ xs) (y ∷ ys) with em x y |  merge xs (y ∷ ys)
merge (x ∷ xs) (y ∷ ys) | inj₁ x₁ | z  = x ∷ z
merge (x ∷ xs) (y ∷ ys) | inj₂ y₁ | _ = y ∷ merge (x ∷ xs) ys 


{-
{- expand to -}
{- ok -}
mutual
  merge : List ℕ -> List ℕ -> List ℕ
  merge [] x₁ = x₁
  merge (x ∷ x₂) [] = x ∷ x₂ 
  merge (x ∷ xs) (y ∷ ys) = merge-aux {x} {y} {xs} {ys} (em x y) (merge  xs (y ∷ ys))
  
  merge-aux : {x y : ℕ}{xs ys : List ℕ} ->  ( x ≤ y ) ⊎ ( y ≤ x ) -> List ℕ  -> List ℕ
  merge-aux {x} {y} {xs} {ys} (inj₁ x₁) z = x ∷  z
  merge-aux {x} {y} {xs} {ys} (inj₂ y₁) z = y ∷ merge (x ∷ xs) ys
-}

